src/VmSemantics.v
@@ -129,10 +129,10 @@ Proof.
 
     assert (
         StVM.st_trace
-           (snd (copland_compile t1 {| st_ev := splitEv s0 e; st_trace := m ++ (k ++ [Term_Defs.split n p]); st_pl := p (*; st_store := o*) |})) =
+           (snd (copland_compile t1 {| st_ev := splitEv_l s e; st_trace := m ++ (k ++ [Term_Defs.split n p]); st_pl := p (*; st_store := o*) |})) =
          m ++
          StVM.st_trace
-         (snd (copland_compile t1 {| st_ev := splitEv s0 e; st_trace := k ++ [Term_Defs.split n p]; st_pl := p; (*st_store := o*) |}))).
+         (snd (copland_compile t1 {| st_ev := splitEv_l s e; st_trace := k ++ [Term_Defs.split n p]; st_pl := p; (*st_store := o*) |}))).
     {
       rewrite <- app_assoc in *. (*Heqp4. *)
       eapply IHt1; eauto.
@@ -145,8 +145,8 @@ Proof.
     subst.
 
     assert (
-         StVM.st_trace (snd (copland_compile t2{| st_ev := splitEv s1 e; st_trace := m ++ st_trace0; st_pl := st_pl0; (*st_store := st_store0*) |})) =
-         m ++ StVM.st_trace (snd (copland_compile t2 {| st_ev := splitEv s1 e; st_trace := st_trace0; st_pl := st_pl0; (*st_store := st_store0*) |}))
+         StVM.st_trace (snd (copland_compile t2{| st_ev := splitEv_r s e; st_trace := m ++ st_trace0; st_pl := st_pl0; (*st_store := st_store0*) |})) =
+         m ++ StVM.st_trace (snd (copland_compile t2 {| st_ev := splitEv_r s e; st_trace := st_trace0; st_pl := st_pl0; (*st_store := st_store0*) |}))
       ).
     eapply IHt2; eauto.
     subst'.
@@ -248,14 +248,14 @@ Proof.
     assert (
         StVM.st_trace
           (snd (copland_compile t1
-                 {| st_ev := splitEv s0 e;
+                 {| st_ev := splitEv_l s e;
                     st_trace := m ++ (k ++ [Term_Defs.split n p]);
                     st_pl := p;
                     (*st_store := map_set o n1 (splitEv s1 e)*) |})) =
          m ++
          StVM.st_trace
          (snd (copland_compile t1
-                               {| st_ev := splitEv s0 e;
+                               {| st_ev := splitEv_l s e;
                                   st_trace := k ++ [Term_Defs.split n p];
                                   st_pl := p;
                                   (*st_store := map_set o n1 (splitEv s1 e)*) |}))).
@@ -272,12 +272,12 @@ Proof.
 
     assert (
         StVM.st_trace (snd (copland_compile t2
-                                            {| st_ev := splitEv s1 e;
+                                            {| st_ev := splitEv_r s e;
                                                st_trace := m ++ st_trace0;
                                                st_pl := p;
                                                (*st_store := st_store4*) |})) =
         m ++ StVM.st_trace (snd (copland_compile t2
-                                                 {| st_ev := splitEv s1 e;
+                                                 {| st_ev := splitEv_r s e;
                                                     st_trace := st_trace0;
                                                     st_pl := p;
                                                     (*st_store := st_store4*) |}))
@@ -740,14 +740,30 @@ Proof.
       repeat do_restl.
       
       econstructor.
-      destruct s0.
+      destruct s.
       ++
         eapply IHt1; eauto.
       ++
         simpl in *.
         eapply IHt1; eauto.
       ++
-        destruct s1.
+        eauto.
+      ++
+        simpl in *.
+        repeat do_pl_immut.
+        subst.
+        destruct s.
+        +++
+          eauto.
+        +++
+          ff.
+          eauto.
+        +++
+          ff.
+          eauto.
+ 
+        (*
+        destruct s.
         +++
           simpl.
           repeat do_pl_immut.
@@ -757,10 +773,53 @@ Proof.
           simpl.
           repeat do_pl_immut.
           subst.
-          eapply IHt2; eauto.
+          eapply IHt2; eauto. *)
 
           
   -
+    do_wf_pieces.
+    df.
+    repeat break_match;
+      try solve_by_inversion;
+      try (df; tauto).
+    +
+      df.
+      annogo.
+      simpl in *.
+      do_suffix blah.
+      do_suffix blah'.
+      destruct_conjs; subst.
+      repeat do_restl.
+      
+      econstructor.
+      destruct s.
+      ++
+        eapply IHt1; eauto.
+      ++
+        simpl in *.
+        eapply IHt1; eauto.
+      ++
+        eauto.
+      ++
+        simpl in *.
+        repeat do_pl_immut.
+        subst.
+        destruct s.
+        +++
+          eauto.
+        +++
+          ff.
+          eauto.
+        +++
+          ff.
+          eauto.
+
+
+
+
+
+(*
+    
     do_wf_pieces.
     repeat (df; dohtac; df).
     dosome.
@@ -825,6 +884,7 @@ Proof.
         eauto.
         eauto.
          *)
+*)
 Defined.
 
 Axiom remote_LTS: forall t n et, 
@@ -856,9 +916,11 @@ Proof.
     
 Defined.
 
-Lemma evshape_split: forall e et s,
+Check splitEv_l.
+
+Lemma evshape_split_l: forall e et s,
     Ev_Shape e et ->
-    Ev_Shape (splitEv s e) (splitEv_T s et).
+    Ev_Shape (splitEv_l s e) (splitEv_T_l s et).
 Proof.
   intros.
   generalizeEverythingElse e.
@@ -866,6 +928,42 @@ Proof.
   -
     invc H.
     destruct s.
+    ff.
+    eauto.
+    ff.
+    eauto.
+    ff.
+    eauto.
+  -
+    invc H.
+    destruct s; ff.
+  -
+    invc H.
+    destruct s; ff.
+  -
+    invc H.
+    destruct s; ff.
+  -
+    invc H.
+    destruct s; ff.
+  -
+    invc H.
+    destruct s; ff.
+    
+Defined.
+
+Lemma evshape_split_r: forall e et s,
+    Ev_Shape e et ->
+    Ev_Shape (splitEv_r s e) (splitEv_T_r s et).
+Proof.
+  intros.
+  generalizeEverythingElse e.
+  induction e; intros.
+  -
+    invc H.
+    destruct s.
+    ff.
+    eauto.
     ff.
     eauto.
     ff.
@@ -979,6 +1077,7 @@ Proof.
   -    
     do_wf_pieces.
     destruct r; destruct s.
+    +
     df.
     vmsts.
     dosome.
@@ -1007,7 +1106,10 @@ Proof.
     Focus 2.
     eassumption.
 
-    eapply evshape_split; eauto.
+    eassumption.
+
+    (*
+    eapply evshape_split_r; eauto. *)
   
     unfold run_cvm in *.
     monad_unfold.
@@ -1022,16 +1124,141 @@ Proof.
     eassumption.
     Focus 2.
     eassumption.
-    eapply evshape_split; eauto.
+    econstructor.
+    (*
+    eapply evshape_split; eauto. *)
+
+    econstructor.
+    eapply stbsrstop.
+    econstructor.
+    +
+          df.
+    vmsts.
+    dosome.
+    df.
+
+    do_suffix blah.
+    do_suffix blah'.
+    destruct_conjs; subst.
+    repeat do_restl.
+    
+    repeat do_pl_immut.
+    subst.
+    repeat rewrite <- app_assoc.
+
+    eapply lstar_tran.
+    econstructor.
+    simpl.
+
+    eapply lstar_transitive.
+    simpl.
+
+    eapply lstar_stbsl.  
+     
+    eapply IHt1.
+    eassumption.
+    Focus 2.
+    eassumption.
+
+    econstructor.
+
+    (*
+
+    eassumption. *)
+
+    (*
+    eapply evshape_split_r; eauto. *)
+  
+    unfold run_cvm in *.
+    monad_unfold.
+
+    eapply lstar_silent_tran.
+    apply stbslstop.
+    
+    eapply lstar_transitive.
+    eapply lstar_stbsr.
+        
+    eapply IHt2.
+    eassumption.
+    Focus 2.
+    eassumption.
+
+    eassumption.
+
+    (*
+    econstructor. *)
+    (*
+    eapply evshape_split; eauto. *)
 
     econstructor.
     eapply stbsrstop.
     econstructor.
 
+    +
+          df.
+    vmsts.
+    dosome.
+    df.
+
+    do_suffix blah.
+    do_suffix blah'.
+    destruct_conjs; subst.
+    repeat do_restl.
+    
+    repeat do_pl_immut.
+    subst.
+    repeat rewrite <- app_assoc.
+
+    eapply lstar_tran.
+    econstructor.
+    simpl.
+
+    eapply lstar_transitive.
+    simpl.
+
+    eapply lstar_stbsl.  
+     
+    eapply IHt1.
+    eassumption.
+    Focus 2.
+    eassumption.
+
+    eassumption.
+
+    (*
+    eapply evshape_split_r; eauto. *)
+  
+    unfold run_cvm in *.
+    monad_unfold.
+
+    eapply lstar_silent_tran.
+    apply stbslstop.
+    
+    eapply lstar_transitive.
+    eapply lstar_stbsr.
+        
+    eapply IHt2.
+    eassumption.
+    Focus 2.
+    eassumption.
+
+    eassumption.
+
+    (*
+    econstructor.
+     *)
+    
+    (*
+    eapply evshape_split; eauto. *)
+
+    econstructor.
+    eapply stbsrstop.
+    econstructor.
 
   -    
     do_wf_pieces.
     destruct r; destruct s.
+    +
     df.
     vmsts.
     dosome.
@@ -1063,7 +1290,11 @@ Proof.
     Focus 2.
     eassumption.
 
+    (*
+
     eapply evshape_split; eauto.
+     *)
+    eassumption.
   
     unfold run_cvm in *.
     monad_unfold.
@@ -1090,13 +1321,168 @@ Proof.
     eassumption.
     Focus 2.
     eassumption.
-    eapply evshape_split; eauto.
+
+    (*
+    eapply evshape_split; eauto. *)
+
+    econstructor.
 
     econstructor.
 
     eapply stbpstop.
 
     econstructor.
+
+        +
+    df.
+    vmsts.
+    dosome.
+    df.
+
+    do_suffix blah.
+    do_suffix blah'.
+    destruct_conjs; subst.
+    repeat do_restl.
+    
+    repeat do_pl_immut.
+    subst.
+    repeat rewrite <- app_assoc.
+
+    eapply lstar_tran.
+    econstructor.
+    simpl.
+
+    eapply lstar_transitive.
+    simpl.
+
+    eapply lstar_stbparl.
+
+    (*
+    eapply lstar_stparl.   *)
+     
+    eapply IHt1.
+    eassumption.
+    Focus 2.
+    eassumption.
+
+    (*
+
+    eapply evshape_split; eauto.
+     *)
+    econstructor.
+  
+    unfold run_cvm in *.
+    monad_unfold.
+
+    eapply lstar_transitive.
+
+    eapply lstar_stbparr.
+
+    (*
+
+    eapply lstar_silent_tran.
+    econstructor.
+
+    apply stbpstop.
+
+
+    
+    apply stbslstop.
+    
+    eapply lstar_transitive.
+    eapply lstar_stbsr. *)
+        
+    eapply IHt2.
+    eassumption.
+    Focus 2.
+    eassumption.
+
+    (*
+    eapply evshape_split; eauto. *)
+
+    eassumption.
+
+    econstructor.
+
+    eapply stbpstop.
+
+    econstructor.
+
+        +
+    df.
+    vmsts.
+    dosome.
+    df.
+
+    do_suffix blah.
+    do_suffix blah'.
+    destruct_conjs; subst.
+    repeat do_restl.
+    
+    repeat do_pl_immut.
+    subst.
+    repeat rewrite <- app_assoc.
+
+    eapply lstar_tran.
+    econstructor.
+    simpl.
+
+    eapply lstar_transitive.
+    simpl.
+
+    eapply lstar_stbparl.
+
+    (*
+    eapply lstar_stparl.   *)
+     
+    eapply IHt1.
+    eassumption.
+    Focus 2.
+    eassumption.
+
+    (*
+
+    eapply evshape_split; eauto.
+     *)
+    eassumption.
+  
+    unfold run_cvm in *.
+    monad_unfold.
+
+    eapply lstar_transitive.
+
+    eapply lstar_stbparr.
+
+    (*
+
+    eapply lstar_silent_tran.
+    econstructor.
+
+    apply stbpstop.
+
+
+    
+    apply stbslstop.
+    
+    eapply lstar_transitive.
+    eapply lstar_stbsr. *)
+        
+    eapply IHt2.
+    eassumption.
+    Focus 2.
+    eassumption.
+
+    (*
+    eapply evshape_split; eauto. *)
+
+    eassumption.
+
+    econstructor.
+
+    eapply stbpstop.
+
+    econstructor.
+ 
 Defined.
 
     (*
